extraction/theories/ScbvEval.v
@@ -27,109 +27,88 @@ Import EAstUtils.
 
 Section seval.
 Context (Σ : global_declarations).
-Inductive eval : term -> term -> Prop :=
-(** Reductions *)
-| eval_box a t t' :
+Inductive seval : term -> term -> Prop :=
+| seval_box_app a t t' :
     eval a tBox ->
     eval t t' ->
     eval (tApp a t) tBox
 
-(** Beta *)
-| eval_beta f na b a a' res :
+| seval_beta f na b a a' res :
     eval f (tLambda na b) ->
     eval a a' ->
     eval (csubst a' 0 b) res ->
     eval (tApp f a) res
 
-(** Let *)
-| eval_zeta na b0 b0' b1 res :
+| seval_zeta na b0 b0' b1 res :
     eval b0 b0' ->
     eval (csubst b0' 0 b1) res ->
     eval (tLetIn na b0 b1) res
 
-(** Case *)
-| eval_iota ind pars discr c args brs res :
+| seval_iota ind pars discr c args brs res :
     eval discr (mkApps (tConstruct ind c) args) ->
     eval (iota_red pars c args brs) res ->
     eval (tCase (ind, pars) discr brs) res
 
-(** Singleton case on a proof *)
-| eval_iota_sing ind pars discr brs n f res :
+| seval_iota_sing ind pars discr brs n f res :
     eval discr tBox ->
     brs = [ (n,f) ] ->
     eval (mkApps f (repeat tBox n)) res ->
     eval (tCase (ind, pars) discr brs) res
 
-(** Fix unfolding, with guard *)
-| eval_fix f mfix idx argsv a av narg fn res :
+| seval_fix f mfix idx argsv a av narg fn res :
     eval f (mkApps (tFix mfix idx) argsv) ->
     eval a av ->
     cunfold_fix mfix idx = Some (narg, fn) ->
     #|argsv| = narg ->
-             is_constructor_app_or_box av ->
-             eval (tApp (mkApps fn argsv) av) res ->
-             eval (tApp f a) res
+    is_constructor_app_or_box av ->
+    eval (tApp (mkApps fn argsv) av) res ->
+    eval (tApp f a) res
 
-(** Fix stuck, with guard *)
-| eval_fix_value f mfix idx argsv a av narg fn :
+| seval_fix_value f mfix idx argsv a av narg fn :
     eval f (mkApps (tFix mfix idx) argsv) ->
     eval a av ->
     cunfold_fix mfix idx = Some (narg, fn) ->
     (#|argsv| <> narg \/ (#|argsv| = narg /\ ~~is_constructor_app_or_box av)) ->
     eval (tApp f a) (tApp (mkApps (tFix mfix idx) argsv) av)
 
-(** CoFix-case unfolding *)
-| red_cofix_case ip mfix idx args narg fn brs res :
+| sred_cofix_case ip mfix idx args narg fn brs res :
     cunfold_cofix mfix idx = Some (narg, fn) ->
     eval (tCase ip (mkApps fn args) brs) res ->
     eval (tCase ip (mkApps (tCoFix mfix idx) args) brs) res
 
-(** CoFix-proj unfolding *)
-| red_cofix_proj p mfix idx args narg fn res :
+| sred_cofix_proj p mfix idx args narg fn res :
     cunfold_cofix mfix idx = Some (narg, fn) ->
     eval (tProj p (mkApps fn args)) res ->
     eval (tProj p (mkApps (tCoFix mfix idx) args)) res
 
-(** Constant unfolding *)
-| eval_delta c decl body (isdecl : declared_constant Σ c decl) res :
+| seval_delta c decl body (isdecl : declared_constant Σ c decl) res :
     decl.(cst_body) = Some body ->
     eval body res ->
     eval (tConst c) res
 
-(** Proj *)
-| eval_proj i pars arg discr args k res :
+| seval_proj i pars arg discr args k res :
     eval discr (mkApps (tConstruct i k) args) ->
     eval (List.nth (pars + arg) args tDummy) res ->
     eval (tProj (i, pars, arg) discr) res
 
-(** Proj *)
-| eval_proj_box i pars arg discr :
+| seval_proj_box i pars arg discr :
     eval discr tBox ->
     eval (tProj (i, pars, arg) discr) tBox
 
-(** Atoms (non redex-producing heads) applied to values are values *)
-| eval_app_cong f f' a a' :
+| seval_app_cong f f' a a' :
     eval f f' ->
     ~~ (isLambda f' || isFixApp f' || isBox f') ->
     eval a a' ->
     eval (tApp f a) (tApp f' a')
 
-| eval_atom_rel i : eval (tRel i) (tRel i)
-| eval_atom_box : eval tBox tBox
-| eval_atom_lambda na body body' :
+| seval_atom_rel i : eval (tRel i) (tRel i)
+| seval_atom_box : eval tBox tBox
+| seval_atom_lambda na body body' :
     eval body body' ->
     eval (tLambda na body) (tLambda na body')
-| eval_atom_construct ind c : eval (tConstruct ind c) (tConstruct ind c)
-| eval_atom_fix defs defs' n :
+| seval_atom_construct ind c : eval (tConstruct ind c) (tConstruct ind c)
+| seval_atom_fix defs defs' n :
 
     Forall2 eval (map dbody defs) (map dbody defs')
 
-(** Evars complicate reasoning due to the embedded substitution, we skip
-      them for now *)
-(* | eval_evar n l l' : *)
-(*     Forall2 eval l l' -> *)
-(*     eval (tEvar n l) (tEvar n l') *)
-
-
-(** Atoms are values (includes abstractions, cofixpoints and constructors) *)
-| eval_atom t : atom t -> eval t t.
+with seval_defs
